\documentclass[
  coursecode={APSC 171},
  assignmentname={Week 9 Material Tutorial Solutions},
  solutiontitle=Solution,
  nodate,
  draft,
  % final,
]{
  ltxanswer%
}

\usepackage{bch-style}

\begin{document}
  \begin{questions}
    \setcounter{question}{35}
    \question{}
    \begin{solution}
      \begin{answerfigure}
        \begin{tikzpicture}[scale=0.75,important line/.style={thick}]
          \draw [opacity=1,important line] (-2,4) -- (2,4) -- (0,0) -- cycle;%big triangle
          \draw [important line,fill=white,opacity=1] (0,4) circle (2cm and 0.4cm);%top of cone
          \draw [fill=blue!20!white,opacity=1] (-1.49,2.98) -- (1.49,2.98) -- (0,0) -- cycle;%smmall triangle
          \draw [fill=blue!10!white,opacity=1,] (0,3) circle (1.49cm and 0.3cm); %top of small cone
          \draw[dashed] (0,0) -- (0,4) --(2,4); %dashed lines
          \draw (1,4.18) node{\scriptsize\(2\)}; % number
          \draw[dashed] (0,2.98) -- (1.49,2.98); %dashed line
          \draw (0.745,3.12) node{\scriptsize\(r\)}; % r
          \draw[|<->|] (2.4,0) -- (2.4,4); %lenght indicator
          \draw[white, fill=white] (2.3,1.75) rectangle (2.5,2.25); %an empty box for the space in middle
          \draw (2.4,2) node{\scriptsize\(5\)}; %a number
          \draw[|<->|] (1.65,0) -- (1.65,2.98); %lenght indicator
          \draw[white, fill=white] (1.45,1.24) rectangle (1.65,1.74);%white rectangle for a space in middle
          \draw (1.65,1.49) node{\scriptsize\(y-7\)};
        \end{tikzpicture}
        \caption{Diagram of the conical portion of the water tank}
        \label{fig:conical-diagram}
      \end{answerfigure}
      Let \(y\) denote the height of any given ``drop'' of water in the tank, where \(y=\qty{0}{\m}\) is the base of the tank and \(y=5+7=\qty{12}{\m}\) is the top of the tank. Then the height of water in the conical portion of the tank is represented by \(y-7\) for \(y \in [7,12]\).

      Let \(W_{S}(y)\) denote the total amount of work done by letting a slice water of thickness \(\Delta y\) in the tank at height \(y\) drain and let \(W_{T}\) be the integral we want to construct. Then
      \begin{align*}
        W_{S}(y)             &= F \cdot d                                                \\
                             &= (m g) (y)                                                \\
                             &= (\rho V) g y                                             \\
                             &= \rho (\pi r^{2} \Delta y) g y                            \\
        \intertext{From Figure~\ref{fig:conical-diagram}, we can represent a water slice's radius using similar triangles:}
        \frac{r}{y-7}        &= \frac{2}{5}                                              \\
        r                    &= \frac{2}{5} (y-7)                                        \\
        \Rightarrow W_{S}(y) &= \rho \pi \biggl(\frac{2}{5}(y-7)\biggr)^{2} g y \Delta y \\
                             &= \frac{4}{25} \rho g \pi y (y-7)^{2} \Delta y             \\
                             &= 1568 \pi y(y - 7)^{2} \Delta y                           \\
        \intertext{\(\therefore\) the total amount of work done can be represented as}
        W_{T}                &= \int W_{S} (y) \dl3y                                     \\
        \alignedbox{         &= 1568 \pi \int_{7}^{12} y(y - 7)^{2} \dl3y}
      \end{align*}
    \end{solution}

    \question{}
    \begin{solution}
      The integrand is a rational function that can undergo partial fraction decomposition to simplify the evaluation of the integral, since \(\deg(4x-2) < \deg(x^{2}-2x+1)\).

      Let \(I\) denote the value of the indefinite integral. Then using partial fraction decomposition yields
      \begin{align*}
        I                                  &= \int \frac{4x-2}{x^{2}-2x+1} \dl3{x}                       \\
                                           &= 2 \int \frac{2x-1}{(x-1)^{2}} \dl3{x}                      \\
                                           &= 2 \int \frac{c_{1}}{x-1} + \frac{c_{2}}{(x-1)^{2}} \dl3{x} \\
        \Rightarrow \frac{2x-1}{(x-1)^{2}} &= \frac{c_{1}}{x-1} + \frac{c_{2}}{(x-1)^{2}}                \\
        2x-1                               &= c_{1}(x-1) + c_{2}                                         \\
        2x-1                               &= c_{1}x - c_{1} + c_{2}                                     \\
        \Rightarrow                        &\begin{cases}
                                              2x = c_{1}x \\
                                              -1 = -c_{1} + c_{2}
                                            \end{cases}                                           \\
        \Rightarrow                        &\begin{cases}
                                              c_{1} = 2 \\
                                              c_{2} = 1
                                            \end{cases}                                                 \\
        \Rightarrow I                      &= 2 \int \frac{2}{x-1} + \frac{1}{(x-1)^{2}} \dl3{x}         \\
        \alignedbox{                       &= 2(2\ln\abs{x-1} - (x-1)^{-1}) + C}.
      \end{align*}
    \end{solution}
  \end{questions}
\end{document}
